lots of reworking and reorganizing to leave some reasonable admits about page_lookup

coq-verification/src/Concrete/PointerLocations.v
@@ -18,6 +18,7 @@ Require Import Coq.Lists.List.
 Require Import Coq.Arith.PeanoNat.
 Require Import Coq.NArith.BinNat.
 Require Import Hafnium.Concrete.Datatypes.
+Require Import Hafnium.Concrete.Parameters.
 Require Import Hafnium.Concrete.Assumptions.Addr.
 Require Import Hafnium.Concrete.Assumptions.ArchMM.
 Require Import Hafnium.Concrete.Assumptions.Constants.
@@ -28,8 +29,44 @@ Require Import Hafnium.Concrete.MM.Datatypes.
 Require Import Hafnium.Util.List.
 Require Import Hafnium.Util.Tactics.
 
+(* TODO : find a different place for this section? *)
+Section AddressMatchesIndices.
+  Definition address_matches_indices_alt stage a idxs : Prop :=
+    firstn (length idxs)
+           (rev
+              (map (fun lvl => get_index stage lvl a)
+                   (seq 0 (S (S (max_level stage)))))) = idxs.
+  Definition address_matches_indices stage a idxs : Prop :=
+    (forall i,
+        i < length idxs ->
+        get_index stage (max_level stage + 1 - i) a = nth_default 0 idxs i).
+
+  Lemma address_matches_indices_iff stage a idxs :
+    address_matches_indices_alt stage a idxs <-> address_matches_indices stage a idxs.
+  Admitted.
+
+  Definition address_matches_indices_alt_dec stage a idxs :
+    {address_matches_indices_alt stage a idxs} + {~ address_matches_indices_alt stage a idxs}.
+  Proof.
+    cbv [address_matches_indices_alt].
+    apply list_eq_dec, Nat.eq_dec.
+  Defined.
+
+  Definition address_matches_indices_dec stage a idxs :
+    {address_matches_indices stage a idxs} + {~ address_matches_indices stage a idxs}.
+  Proof.
+    destruct (address_matches_indices_alt_dec stage a idxs);
+      rewrite address_matches_indices_iff in *; solver.
+  Defined.
+End AddressMatchesIndices.
+
+Section LevelFromIndices.
+  Definition level_from_indices stage (idxs : list nat) : nat :=
+    max_level stage + 2 - length idxs.
+End LevelFromIndices.
+
 Section PointerLocations.
-  Context (ptable_deref : ptable_pointer -> mm_page_table).
+  Context (deref : ptable_pointer -> mm_page_table).
 
   (* We haven't formalized anywhere that pointers don't repeat, so we return a
      list of all locations where the provided pointer exists even though we
@@ -45,7 +82,7 @@ Section PointerLocations.
       if ptable_pointer_eq_dec root ptr
       then cons nil nil
       else
-        let ptable := ptable_deref root in
+        let ptable := deref root in
         flat_map
           (fun index =>
              match get_entry ptable index with
@@ -102,13 +139,16 @@ Section PointerLocations.
   (* This section includes some definitions which use information from the
      concrete parameters *)
   Section with_concrete_params.
-    Context (vm_ptables : list mm_ptable) (haf_ptable : mm_ptable) (ppool : mpool).
+    Context {cp : concrete_params}.
 
-    Inductive has_location : ptable_pointer -> pointer_location ppool -> Prop :=
+    Let vm_ptables := map vm_ptable vms.
+
+    Inductive has_location {ppool : mpool}
+      : ptable_pointer -> pointer_location ppool -> Prop :=
     | has_table_loc_stage1 :
         forall idxs ptr,
-          In idxs (index_sequences_to_pointer ptr haf_ptable Stage1) ->
-          has_location ptr (table_loc ppool haf_ptable idxs)
+          In idxs (index_sequences_to_pointer ptr hafnium_ptable Stage1) ->
+          has_location ptr (table_loc ppool hafnium_ptable idxs)
     | has_table_loc_stage2 :
         forall root_ptable idxs ptr,
           In root_ptable vm_ptables ->
@@ -120,181 +160,277 @@ Section PointerLocations.
           has_location ptr (mpool_loc ppool)
     .
 
-    (* TODO: just guessing that this might come in handy; remove if unused *)
-    Lemma table_locations_exclusive ptr1 ptr2 root_ptable idxs :
-      has_location ptr1 (table_loc ppool root_ptable idxs) ->
-      has_location ptr2 (table_loc ppool root_ptable idxs) ->
-      ptr1 = ptr2.
-    Admitted.
-
     (* every ptable_pointer has at most one location *)
-    Definition locations_exclusive : Prop :=
+    Definition locations_exclusive (ppool : mpool) : Prop :=
       forall ptr loc1 loc2,
-        has_location ptr loc1 -> has_location ptr loc2 -> loc1 = loc2.
+        @has_location ppool ptr loc1 -> @has_location ppool ptr loc2 -> loc1 = loc2.
   End with_concrete_params.
 
-  Lemma index_sequences_to_pointer''_root ptr level :
-    0 < level ->
-    In nil (index_sequences_to_pointer'' ptr ptr level).
-  Proof.
-    destruct level; [solver|]; intros.
-    cbn [index_sequences_to_pointer''].
-    break_match; solver.
-  Qed.
 
-  Lemma index_sequences_to_pointer'_nth_default root_list stage :
-    forall i j k,
-      i < length root_list ->
-      k = i + j ->
-      In (k :: nil)
-         (index_sequences_to_pointer'
-            (nth_default_oobe root_list i) j root_list stage).
-  Proof.
-    cbv [nth_default_oobe]. pose proof (max_level_pos stage).
-    induction root_list; destruct i; cbn [length index_sequences_to_pointer'];
-      repeat match goal with
-             | _ => progress basics
-             | _ => progress autorewrite with push_nth_default
-             | _ => rewrite Nat.add_0_l
-             | _ => apply in_or_app
-             | _ => left; apply in_map, index_sequences_to_pointer''_root; solver
-             | _ => right; apply IHroot_list; solver
-             | _ => solver
-             end.
-  Qed.
+  Section Proofs.
+    Lemma index_sequences_to_pointer''_root ptr level :
+      0 < level ->
+      In nil (index_sequences_to_pointer'' ptr ptr level).
+    Proof.
+      destruct level; [solver|]; intros.
+      cbn [index_sequences_to_pointer''].
+      break_match; solver.
+    Qed.
 
-  (* Helper lemma for [nth_error_index_sequences_root] *)
-  Lemma nth_error_index_sequences_root' root_ptrs stage ptr :
-    forall i root_index,
-      nth_error root_ptrs i = Some ptr ->
-      In (cons (root_index + i) nil)
-         (index_sequences_to_pointer' ptr root_index root_ptrs stage).
-  Proof.
-    induction root_ptrs; [ intros *; rewrite nth_error_nil; solver | ].
-    destruct i; cbn [nth_error index_sequences_to_pointer']; basics.
-    { apply in_or_app; left. rewrite Nat.add_0_r. apply in_map.
-      apply index_sequences_to_pointer''_root; solver. }
-    { apply in_or_app; right. rewrite <-Nat.add_succ_comm.
-      solver. }
-  Qed.
+    Lemma index_sequences_to_pointer'_nth_default root_list stage :
+      forall i j k,
+        i < length root_list ->
+        k = i + j ->
+        In (k :: nil)
+           (index_sequences_to_pointer'
+              (nth_default_oobe root_list i) j root_list stage).
+    Proof.
+      cbv [nth_default_oobe]. pose proof (max_level_pos stage).
+      induction root_list; destruct i; cbn [length index_sequences_to_pointer'];
+        repeat match goal with
+               | _ => progress basics
+               | _ => progress autorewrite with push_nth_default
+               | _ => rewrite Nat.add_0_l
+               | _ => apply in_or_app
+               | _ => left; apply in_map, index_sequences_to_pointer''_root; solver
+               | _ => right; apply IHroot_list; solver
+               | _ => solver
+               end.
+    Qed.
 
-  (* If you're searching for the index sequences leading to [ptr], and [ptr] is
+    (* Helper lemma for [nth_error_index_sequences_root] *)
+    Lemma nth_error_index_sequences_root' root_ptrs stage ptr :
+      forall i root_index,
+        nth_error root_ptrs i = Some ptr ->
+        In (cons (root_index + i) nil)
+           (index_sequences_to_pointer' ptr root_index root_ptrs stage).
+    Proof.
+      induction root_ptrs; [ intros *; rewrite nth_error_nil; solver | ].
+      destruct i; cbn [nth_error index_sequences_to_pointer']; basics.
+      { apply in_or_app; left. rewrite Nat.add_0_r. apply in_map.
+        apply index_sequences_to_pointer''_root; solver. }
+      { apply in_or_app; right. rewrite <-Nat.add_succ_comm.
+        solver. }
+    Qed.
+
+    (* If you're searching for the index sequences leading to [ptr], and [ptr] is
      a pointer to the root page table at index [i] in the root table list, then
      the resulting index sequences will include (cons i nil).*)
-  Lemma nth_error_index_sequences_root root_ptable i stage ptr :
-    nth_error (ptr_from_va (va_from_pa (root root_ptable))) i = Some ptr ->
-    In (cons i nil) (index_sequences_to_pointer ptr root_ptable stage).
-  Proof.
-    cbv [index_sequences_to_pointer]; intro Hnth.
-    eapply nth_error_index_sequences_root' with (root_index:=0) in Hnth.
-    rewrite Nat.add_0_l in Hnth. solver.
-  Qed.
+    Lemma nth_error_index_sequences_root root_ptable i stage ptr :
+      nth_error (ptr_from_va (va_from_pa (root root_ptable))) i = Some ptr ->
+      In (cons i nil) (index_sequences_to_pointer ptr root_ptable stage).
+    Proof.
+      cbv [index_sequences_to_pointer]; intro Hnth.
+      eapply nth_error_index_sequences_root' with (root_index:=0) in Hnth.
+      rewrite Nat.add_0_l in Hnth. solver.
+    Qed.
 
-  Lemma index_sequences_not_nil' ptr root_ptrs stage :
-    Exists (fun root_ptr =>
-              index_sequences_to_pointer''
-                ptr root_ptr (max_level stage + 1) <> nil)
-        root_ptrs ->
-    forall root_index,
-      index_sequences_to_pointer' ptr root_index root_ptrs stage <> nil.
-  Proof.
-    induction 1; cbn [index_sequences_to_pointer'];
-      eauto using app_not_nil_l, app_not_nil_r, map_not_nil.
-  Qed.
+    Lemma index_sequences_not_nil' ptr root_ptrs stage :
+      Exists (fun root_ptr =>
+                index_sequences_to_pointer''
+                  ptr root_ptr (max_level stage + 1) <> nil)
+             root_ptrs ->
+      forall root_index,
+        index_sequences_to_pointer' ptr root_index root_ptrs stage <> nil.
+    Proof.
+      induction 1; cbn [index_sequences_to_pointer'];
+        eauto using app_not_nil_l, app_not_nil_r, map_not_nil.
+    Qed.
 
-  Lemma index_sequences_not_nil ptr root_ptable stage :
-    Exists (fun root_ptr =>
-              index_sequences_to_pointer''
-                ptr root_ptr (max_level stage + 1) <> nil)
-        (ptr_from_va (va_from_pa (root root_ptable))) ->
-    index_sequences_to_pointer ptr root_ptable stage <> nil.
-  Proof.
-    cbv [index_sequences_to_pointer]. basics.
-    apply index_sequences_not_nil'; eauto.
-  Qed.
+    Lemma index_sequences_not_nil ptr root_ptable stage :
+      Exists (fun root_ptr =>
+                index_sequences_to_pointer''
+                  ptr root_ptr (max_level stage + 1) <> nil)
+             (ptr_from_va (va_from_pa (root root_ptable))) ->
+      index_sequences_to_pointer ptr root_ptable stage <> nil.
+    Proof.
+      cbv [index_sequences_to_pointer]. basics.
+      apply index_sequences_not_nil'; eauto.
+    Qed.
 
-  Lemma get_entry_index_sequences level :
-    forall i root_ptr e,
-      0 < level ->
-      get_entry (ptable_deref root_ptr) i = Some e ->
-      arch_mm_pte_is_table e level = true ->
-      index_sequences_to_pointer''
-        (ptable_pointer_from_address (arch_mm_table_from_pte e level))
-        root_ptr (S level) <> nil.
-  Proof.
-    basics; cbn [index_sequences_to_pointer''];
-      match goal with
-      | H : get_entry _ _ = Some _ |- _ =>
-        pose proof H; cbv [get_entry] in H; apply nth_error_Some_range in H
-      end;
-      repeat match goal with
-             | _ => progress basics
-             | H : get_entry _ _ = Some _ |- _ => rewrite H
-             | _ => break_match
-             | _ => apply flat_map_not_nil with (a:=i)
-             | _ => apply in_seq; solver
-             | _ => solver
-             | _ => solve [eauto using map_not_nil, In_not_nil,
-                           index_sequences_to_pointer''_root]
-             end.
-  Qed.
+    Lemma get_entry_index_sequences level :
+      forall i root_ptr e,
+        0 < level ->
+        get_entry (deref root_ptr) i = Some e ->
+        arch_mm_pte_is_table e level = true ->
+        index_sequences_to_pointer''
+          (ptable_pointer_from_address (arch_mm_table_from_pte e level))
+          root_ptr (S level) <> nil.
+    Proof.
+      basics; cbn [index_sequences_to_pointer''];
+        match goal with
+        | H : get_entry _ _ = Some _ |- _ =>
+          pose proof H; cbv [get_entry] in H; apply nth_error_Some_range in H
+        end;
+        repeat match goal with
+               | _ => progress basics
+               | H : get_entry _ _ = Some _ |- _ => rewrite H
+               | _ => break_match
+               | _ => apply flat_map_not_nil with (a:=i)
+               | _ => apply in_seq; solver
+               | _ => solver
+               | _ => solve [eauto using map_not_nil, In_not_nil,
+                             index_sequences_to_pointer''_root]
+               end.
+    Qed.
 
-  Lemma page_lookup'_proper deref2 level stage :
-    forall root_ptr,
+    Lemma page_lookup'_proper deref2 level stage :
+      forall root_ptr,
+        (forall ptr,
+            index_sequences_to_pointer'' ptr root_ptr level <> nil ->
+            deref ptr = deref2 ptr) ->
+        forall a,
+          page_lookup' deref a (deref root_ptr) level stage
+          = page_lookup' deref2 a (deref root_ptr) level stage.
+    Proof.
+      induction level; cbn [page_lookup'];
+        [ | destruct (Nat.eq_dec level 0); [ basics; reflexivity | ] ];
+        repeat match goal with
+               | _ => progress basics
+               | _ => break_match
+               | H : _ |- _ =>
+                 rewrite <-H; [ | eapply get_entry_index_sequences; solver ]
+               | H : context [deref _ = deref2 _] |- _ => apply H
+               | _ => apply IHlevel
+               | _ => solver
+               end.
+      cbn [index_sequences_to_pointer''].
+      break_match; [ solver | ].
+      cbv [get_entry] in *.
+      match goal with H : _ |- _ =>
+                      pose proof H;
+                        apply nth_error_Some_range in H
+      end.
+      match goal with H : context [get_index ?s ?l ?addr] |- _ =>
+                      eapply flat_map_not_nil with (a0:=get_index s l addr);
+                        [ apply in_seq; solver | ]
+      end.
+      repeat break_match; try solver; [ ].
+      apply map_not_nil; solver.
+    Qed.
+
+    Lemma page_lookup_proper deref2 root_ptable stage :
       (forall ptr,
-          index_sequences_to_pointer'' ptr root_ptr level <> nil ->
-          ptable_deref ptr = deref2 ptr) ->
+          index_sequences_to_pointer ptr root_ptable stage <> nil ->
+          deref ptr = deref2 ptr) ->
       forall a,
-        page_lookup' ptable_deref a (ptable_deref root_ptr) level stage
-        = page_lookup' deref2 a (ptable_deref root_ptr) level stage.
-  Proof.
-    induction level; cbn [page_lookup'];
-      [ | destruct (Nat.eq_dec level 0); [ basics; reflexivity | ] ];
-      repeat match goal with
-             | _ => progress basics
-             | _ => break_match
-             | H : _ |- _ =>
-               rewrite <-H; [ | eapply get_entry_index_sequences; solver ]
-             | H : context [ptable_deref _ = deref2 _] |- _ => apply H
-             | _ => apply IHlevel
-             | _ => solver
-             end.
-    cbn [index_sequences_to_pointer''].
-    break_match; [ solver | ].
-    cbv [get_entry] in *.
-    match goal with H : _ |- _ =>
-                    pose proof H;
-                      apply nth_error_Some_range in H
-    end.
-    match goal with H : context [get_index ?s ?l ?addr] |- _ =>
-                    eapply flat_map_not_nil with (a0:=get_index s l addr);
-                      [ apply in_seq; solver | ]
-    end.
-    repeat break_match; try solver; [ ].
-    apply map_not_nil; solver.
-  Qed.
+        page_lookup deref root_ptable stage a = page_lookup deref2 root_ptable stage a.
+    Proof.
+      cbv [page_lookup];
+        repeat match goal with
+               | _ => progress basics
+               | H : _ = Some _ |- _ =>
+                 pose proof (nth_error_In _ _ H);
+                   eapply nth_error_index_sequences_root in H;
+                   [ | solver .. ]
+               | H : context [deref _ = deref2 _] |- _ => rewrite <-H by solver
+               | H : context [deref _ = deref2 _] |- _ =>
+                 apply H; apply index_sequences_not_nil
+               | _ => apply page_lookup'_proper
+               | _ => rewrite Exists_exists
+               | _ => break_match
+               | _ => solver
+               end.
+    Qed.
 
-  Lemma page_lookup_proper deref2 root_ptable stage :
-    (forall ptr,
-        index_sequences_to_pointer ptr root_ptable stage <> nil ->
-        ptable_deref ptr = deref2 ptr) ->
-    forall a,
-      page_lookup ptable_deref root_ptable stage a = page_lookup deref2 root_ptable stage a.
-  Proof.
-    cbv [page_lookup];
-      repeat match goal with
-             | _ => progress basics
-             | H : _ = Some _ |- _ =>
-               pose proof (nth_error_In _ _ H);
-                 eapply nth_error_index_sequences_root in H;
-                 [ | solver .. ]
-             | H : context [ptable_deref _ = deref2 _] |- _ => rewrite <-H by solver
-             | H : context [ptable_deref _ = deref2 _] |- _ =>
-               apply H; apply index_sequences_not_nil
-             | _ => apply page_lookup'_proper
-             | _ => rewrite Exists_exists
-             | _ => break_match
-             | _ => solver
-             end.
-  Qed.
+    (* TODO: clean up WIP proofs, move definition of page_table_lookup elsewhere *)
+    (*** The below proofs are a work in progress to connect index_sequences_to_pointer with page_lookup ***)
+
+    Section PageTableLookup.
+      (* TODO: remove if unused *)
+      (* Look up the page table that corresponds to the given indices *)
+      Fixpoint page_table_lookup' root_ptr (idxs : list nat) level : option ptable_pointer :=
+        match idxs with
+        | nil => Some root_ptr
+        | cons i idxs' =>
+          let table := deref root_ptr in
+          match get_entry table i with
+          | Some pte =>
+            if arch_mm_pte_is_table pte level
+            then
+              let next_ptr := ptable_pointer_from_address (arch_mm_table_from_pte pte level) in
+              page_table_lookup' next_ptr idxs' (level - 1)
+            else Some root_ptr
+          | None => None
+          end
+        end.
+      Definition page_table_lookup root_ptable idxs stage : option ptable_pointer :=
+        let root_tables := ptr_from_va (va_from_pa (root root_ptable)) in
+        match idxs with
+        | nil => None
+        | cons i idxs' =>
+          match nth_error root_tables i with
+          | Some table_ptr => page_table_lookup' table_ptr idxs' (max_level stage)
+          | None => None
+          end
+        end.
+    End PageTableLookup.
+
+    (* TODO: remove if unused *)
+    Lemma page_table_lookup_equiv root_ptable idxs stage a ptr :
+      address_matches_indices stage a idxs ->
+      page_table_lookup root_ptable idxs stage = Some ptr ->
+      page_lookup deref root_ptable stage a
+      = page_lookup' deref a (deref ptr) (level_from_indices stage idxs) stage.
+    Admitted.
+
+    Section with_concrete_params.
+      Context {cp : concrete_params}.
+
+      Definition root_ptable_matches_stage root_ptable stage : Prop :=
+        match stage with
+        | Stage1 => root_ptable = hafnium_ptable
+        | Stage2 => In root_ptable (map vm_ptable vms)
+        end.
+
+      Lemma has_location_index_sequence ppool ptr root_ptable idxs stage :
+        root_ptable_matches_stage root_ptable stage ->
+        ~ In hafnium_ptable (map vm_ptable vms) ->
+        has_location ptr (table_loc ppool root_ptable idxs) ->
+        In idxs (index_sequences_to_pointer ptr root_ptable stage).
+      Proof.
+        intros.
+        match goal with H : context [has_location] |- _ =>
+                        invert H end; destruct stage; try solver.
+      Qed.
+
+      (* TODO: remove if unused *)
+      Lemma has_location_step
+            ppool root_ptable stage idxs ptr i level e :
+        root_ptable_matches_stage root_ptable stage ->
+        has_location ptr (table_loc ppool root_ptable idxs) ->
+        level = level_from_indices stage idxs ->
+        get_entry (deref ptr) i = Some e ->
+        arch_mm_pte_is_table e level = true ->
+        let next_ptr :=
+            ptable_pointer_from_address (arch_mm_table_from_pte e level) in
+        has_location next_ptr (table_loc ppool root_ptable (idxs ++ cons i nil)).
+      Admitted.
+
+      (* TODO: remove if unused *)
+      Lemma has_location_table_lookup ppool ptr root_ptable idxs stage :
+        has_location ptr (table_loc ppool root_ptable idxs) ->
+        page_table_lookup root_ptable idxs stage = Some ptr.
+      Admitted.
+
+      (* TODO: remove if unused *)
+      Lemma page_lookup_from_location root_ptable idxs ppool stage a ptr :
+        has_location ptr (table_loc ppool root_ptable idxs) ->
+        address_matches_indices stage a idxs ->
+        page_lookup deref root_ptable stage a
+        = page_lookup' deref a (deref ptr) (level_from_indices stage idxs) stage.
+      Proof.
+        intros;
+          match goal with H : _ |- _ =>  eapply has_location_table_lookup in H end.
+        eapply page_table_lookup_equiv; eauto.
+      Qed.
+
+      (* TODO: just guessing that this might come in handy; remove if unused *)
+      Lemma table_locations_exclusive ppool ptr1 ptr2 root_ptable idxs :
+        has_location ptr1 (table_loc ppool root_ptable idxs) ->
+        has_location ptr2 (table_loc ppool root_ptable idxs) ->
+        ptr1 = ptr2.
+      Admitted.
+    End with_concrete_params.
+  End Proofs.
 End PointerLocations.
