coq-verification/src/Concrete/Parameters.v
@@ -1,0 +1,68 @@
+
+(*
+ * Copyright 2019 Jade Philipoom
+ *
+ * Licensed under the Apache License, Version 2.0 (the "License");
+ * you may not use this file except in compliance with the License.
+ * You may obtain a copy of the License at
+ *
+ *     https://www.apache.org/licenses/LICENSE-2.0
+ *
+ * Unless required by applicable law or agreed to in writing, software
+ * distributed under the License is distributed on an "AS IS" BASIS,
+ * WITHOUT WARRANTIES OR CONDITIONS OF ANY KIND, either express or implied.
+ * See the License for the specific language governing permissions and
+ * limitations under the License.
+ *)
+
+Require Import Coq.Lists.List.
+Require Import Hafnium.Concrete.Datatypes.
+Require Import Hafnium.Concrete.Assumptions.Addr.
+Require Import Hafnium.Concrete.Assumptions.ArchMM.
+Require Import Hafnium.Concrete.Assumptions.Constants.
+Require Import Hafnium.Concrete.Assumptions.Datatypes.
+Require Import Hafnium.Concrete.MM.Datatypes.
+
+(*** This file defines the starting parameters for the concrete state. It is kept
+   separate so that definitions using concrete_params can be used in State.v ***)
+
+Record vm :=
+  {
+    vm_ptable : mm_ptable;
+    vm_id : nat;
+  }.
+
+(* N.B. there can be multiple page tables at the root level *)
+Definition vm_root_tables (v : vm) : list ptable_pointer :=
+  ptr_from_va (va_from_pa v.(vm_ptable).(root)).
+
+(* starting parameters -- don't change *)
+Class concrete_params :=
+  {
+    vms : list vm;
+    hafnium_ptable : mm_ptable;
+  }.
+
+(* N.B. there can be multiple page tables at the root level *)
+Definition hafnium_root_tables {cp : concrete_params} : list ptable_pointer :=
+  ptr_from_va (va_from_pa hafnium_ptable.(root)).
+
+Definition all_root_ptables {cp : concrete_params} : list mm_ptable :=
+  hafnium_ptable :: map vm_ptable vms.
+
+Definition all_root_ptable_pointers {cp : concrete_params}
+  : list ptable_pointer := hafnium_root_tables ++ flat_map vm_root_tables vms.
+
+Class params_valid {cp : concrete_params} :=
+  {
+    correct_number_of_root_tables_stage1 :
+      length (ptr_from_va (va_from_pa (hafnium_ptable.(root))))
+      = arch_mm_stage1_root_table_count;
+    correct_number_of_root_tables_stage2 :
+      forall t,
+        In t (map vm_ptable vms) ->
+        length (ptr_from_va (va_from_pa t.(root)))
+        = arch_mm_stage2_root_table_count;
+    no_duplicate_ptables : NoDup all_root_ptables;
+    no_duplicate_ids : NoDup (map vm_id vms)
+  }.
